Logic/Modal/Standard/Kripke/Soundness.lean
@@ -5,46 +5,20 @@ namespace LO.Modal.Standard.Kripke
 
 variable {W α : Type*}
 variable {Λ : AxiomSet α}
+variable [Inhabited α]
 
 open Deduction
 open Formula Formula.Kripke
 
-lemma sound (d : Λ ⊢ p) : 𝔽(Λ, W) ⊧ p := by
+lemma sound_on_frameclass (d : Λ ⊢ p) : 𝔽(Λ) ⊧ p := by
   induction d with
   | maxm h => exact validOnAxiomSetFrameClass_axiom h;
   | mdp _ _ ihpq ihp =>
-    intro F hF V w;
-    have := ihpq F hF V w;
-    have := ihp F hF V w;
-    simp_all;
+    intro W _ F hF V w;
+    exact (Semantics.Tarski.realize_imp.mp $ ihpq W F hF V w) (ihp W F hF V w);
   | nec _ ih =>
-    intro F hF V w w' _;
-    exact ih F hF V w';
-  | disj₃ =>
-    intro _ _;
-    simp_all [ValidOnFrameClass, ValidOnFrame, ValidOnModel];
-    intros; rename_i hpr hqr hpq;
-    cases hpq with
-    | inl hp => exact hpr hp;
-    | inr hq => exact hqr hq;
-  | _ =>
-    intro _ _;
-    simp_all [ValidOnFrameClass, ValidOnFrame, ValidOnModel];
-
-lemma sound! : Λ ⊢! p → 𝔽(Λ, W) ⊧ p := λ ⟨d⟩ => sound d
-
-instance : Sound Λ 𝔽(Λ, W) := ⟨sound!⟩
-
-
-lemma sound_on_model {M : Model W α} [M ⊧* Λ] (d : Λ ⊢ p) : M ⊧ p := by
-  induction d with
-  | maxm h => exact Semantics.RealizeSet.realize _ h
-  | mdp _ _ ihpq ihp =>
-    intro w;
-    exact (Semantics.Tarski.realize_imp.mp $ ihpq w) (ihp w);
-  | nec _ ih =>
-    intro w w' _;
-    exact ih w';
+    intro W _ F hF V w w' _;
+    exact ih W F hF V w';
   | disj₃ =>
     simp_all [ValidOnFrameClass, ValidOnFrame, ValidOnModel];
     intros; rename_i hpr hqr hpq;
@@ -53,30 +27,17 @@ lemma sound_on_model {M : Model W α} [M ⊧* Λ] (d : Λ ⊢ p) : M ⊧ p := by
     | inr hq => exact hqr hq;
   | _ => simp_all [ValidOnFrameClass, ValidOnFrame, ValidOnModel];
 
-lemma sound_on_model! {M : Model W α} [M ⊧* Λ] : Λ ⊢! p → M ⊧ p := λ ⟨d⟩ => sound_on_model d
+lemma sound!_on_frameclass : Λ ⊢! p → 𝔽(Λ) ⊧ p := λ ⟨d⟩ => sound_on_frameclass d
 
-instance {M : Model W α} [M ⊧* Λ] : Sound Λ M := ⟨sound_on_model!⟩
+instance : Sound Λ (𝔽(Λ)) := ⟨sound!_on_frameclass⟩
 
+lemma unprovable_bot [ne : FrameClass.Nonempty 𝔽(Λ)] : Λ ⊬! ⊥ := by
+  intro h;
+  obtain ⟨W, _, F, hf⟩ := ne.existsi;
+  simpa [ValidOnFrame ,ValidOnModel] using sound!_on_frameclass h _ F hf;
 
-lemma sound_on_frame {F : Frame W α} [F ⊧* Λ] (d : Λ ⊢ p) : F ⊧ p := by
-  induction d with
-  | maxm h => exact Semantics.realizeSet_iff.mp (by assumption) h;
-  | mdp _ _ ihpq ihp =>
-    intro V w;
-    exact (Semantics.Tarski.realize_imp.mp $ ihpq V w) (ihp V w);
-  | nec _ ih =>
-    intro V w w' _;
-    exact ih V w';
-  | disj₃ =>
-    simp_all [ValidOnFrameClass, ValidOnFrame, ValidOnModel];
-    intros; rename_i hpr hqr hpq;
-    cases hpq with
-    | inl hp => exact hpr hp;
-    | inr hq => exact hqr hq;
-  | _ => simp_all [ValidOnFrameClass, ValidOnFrame, ValidOnModel];
+instance [FrameClass.Nonempty 𝔽(Λ)] : System.Consistent Λ := System.Consistent.of_unprovable unprovable_bot
 
-lemma sound_on_frame! {F : Frame W α} [F ⊧* Λ] : Λ ⊢! p → F ⊧ p := λ ⟨d⟩ => sound_on_frame d
-
-instance {F : Frame W α} [F ⊧* Λ] : Sound Λ F := ⟨sound_on_frame!⟩
+instance : System.Consistent (𝐊 : AxiomSet α) := inferInstance
 
 end LO.Modal.Standard.Kripke
